bidirectional/theories/BDToPCUIC.v
@@ -1,0 +1,232 @@
+From Coq Require Import Bool List Arith Lia.
+From MetaCoq.Template Require Import config utils monad_utils.
+From MetaCoq.PCUIC Require Import PCUICAst PCUICLiftSubst PCUICTyping.
+From MetaCoq.PCUIC Require Import PCUICPrincipality PCUICClosed PCUICValidity PCUICCumulativity PCUICSR.
+From MetaCoq.Bidirectional Require Import BDEnvironmentTyping BDTyping.
+
+Require Import ssreflect.
+From Equations Require Import Equations.
+Require Import Equations.Prop.DepElim.
+
+
+Module PT := PCUIC.PCUICTyping.
+Module BD := Bidirectional.BDTyping.
+
+Section BDToPCUICTyping.
+
+  Definition Pcheck `{checker_flags} Σ Γ t T :=
+    Σ ;;; Γ |- t : T.
+
+  Definition Pinfer `{checker_flags} Σ Γ t T :=
+    Σ ;;; Γ |- t : T.
+
+  Definition Psort `{checker_flags} Σ Γ t u :=
+    Σ ;;; Γ |- t : (tSort u).
+
+  Definition Pprod `{checker_flags} Σ Γ t na A B :=
+    Σ ;;; Γ |- t : tProd na A B.
+
+  Definition Pind `{checker_flags} Σ Γ ind t u args :=
+    Σ ;;; Γ |- t : mkApps (tInd ind u) args.
+
+  Definition PΓ `{checker_flags} Σ Γ (wfΓ : wf_local Σ Γ) :=
+    PT.wf_local Σ Γ.
+
+Lemma bd_wf `{checker_flags} Σ : Forall_decls_sorting Pcheck Psort Σ -> PT.wf Σ.
+Proof.
+   intros wfΣ. induction wfΣ.
+  all: constructor.
+  - assumption.
+  - assumption.
+  - constructor ; intuition.
+  - destruct d as [[? [] ?]|].
+    + assumption.
+    + destruct o0. eexists.
+      eauto.
+    + destruct o0.
+      constructor ; intuition.
+      * induction onInductives.
+        all: constructor ; auto.
+        destruct p.
+        unshelve econstructor.
+        -- exact ind_indices.
+        -- exact ind_sort.
+        -- eapply map.
+           2: exact ind_cshapes.
+           intros [].
+           constructor ; auto.
+        -- assumption.
+        -- assumption.
+        -- apply All2_map_right.
+           eapply All2_impl.
+           1: exact onConstructors.
+           intros [[] ?] [] [] ; simpl in *. constructor ; auto ; simpl in *.
+           ++ match goal with |- PT.type_local_ctx _ _ ?ctx _ _ => remember ctx as Γ' end.
+              clear -on_cargs.
+              induction cshape_args as [|[? []]].
+              1: auto.
+              ** destruct on_cargs as [[] ].
+                 repeat split ; auto.
+              ** destruct on_cargs. repeat split ; auto.
+           ++  match goal with |- PT.ctx_inst _ _ ?ctx _ _ => remember ctx as Γ' end.
+               clear -on_cindices.
+               induction on_cindices.
+               all: constructor.
+               all: assumption.
+           ++ clear - on_ctype_positive.
+              cbn in on_ctype_positive |- *.
+              induction on_ctype_positive.
+              all: constructor ; auto.
+              clear - p. induction p.
+              ** constructor ; assumption.
+              ** constructor 2 ; auto.
+              ** constructor 3 ; auto.
+              ** constructor 4 ; auto.
+           ++ clear - on_ctype_variance.
+              intros v e.
+              specialize (on_ctype_variance v e).
+              unfold respects_variance in on_ctype_variance.
+              unfold PT.respects_variance.
+              destruct (PCUICEnvironment.ind_universes m) ; simpl in *.
+              ** destruct on_ctype_variance as [a ?] ; split ; auto.
+                 induction a ; intuition.
+              ** destruct cst ; intuition.
+                 unfold level_var_instance in a ; unfold PT.level_var_instance.
+                 match goal with |- PT.All2_local_env (PT.on_decl ?Q) ?ctx ?ctx' =>
+                  remember ctx as Γ ; remember ctx' as Γ' end.
+                  clear - a.
+                  induction a.
+                  all: constructor ; auto.
+            
+        -- intros projs ; specialize (onProjections projs).
+           clear - onProjections.
+           induction ind_cshapes.
+           1: auto.
+           simpl in *.
+           destruct ind_cshapes.
+           { destruct a. simpl in *.
+             destruct onProjections. constructor ; intuition. }
+           assumption.
+
+        -- clear -ind_sorts.
+           cbn in *.
+           red in ind_sorts |- *.
+           destruct (universe_family ind_sort).
+           ++ induction ind_cshapes ; auto.
+              simpl in *.
+              destruct ind_cshapes ; auto.
+              destruct a ; auto.
+           ++ destruct ind_sorts. split.
+              { apply Forall_map.
+                eapply Forall_impl. 1: eassumption.
+                intros [] ? ; assumption. }
+              destruct indices_matter ; auto.
+              induction ind_indices as [|[? []]].
+              1: auto.
+              ** destruct y as [[] ].
+                 repeat split ; auto.
+              ** destruct y. repeat split ; auto.
+           ++ destruct ind_sorts. split.
+              { apply Forall_map.
+                eapply Forall_impl. 1: eassumption.
+                intros [] ? ; assumption. }
+              destruct indices_matter ; auto.
+              induction ind_indices as [|[? []]].
+              1: auto.
+              ** destruct y as [[] ].
+                 repeat split ; auto.
+              ** destruct y. repeat split ; auto.
+      * clear - onParams.
+        induction onParams.
+        all: constructor ; intuition.
+Admitted.
+      
+
+Lemma bd_wf_local `{checker_flags} Σ Γ (all: wf_local Σ Γ) :
+  BD.All_local_env_over_sorting checking infering_sort 
+    (fun Σ Γ _ t T _ => Pcheck Σ Γ t T)
+    (fun Σ Γ _ t u _ => Psort Σ Γ t u) 
+    Σ Γ all ->
+  PT.wf_local Σ Γ.
+Proof.
+  intros allo ; induction allo.
+  all: constructor.
+  1,3: assumption.
+  all: red.
+  - simpl in t0. eexists.
+     eassumption.
+  - destruct t0. eexists.
+    eassumption.
+  - destruct t0.
+    assumption.
+Qed.   
+  
+Theorem Bidirectional_to_PCUIC `{cf : checker_flags} : env_prop Pcheck Pinfer Psort Pprod Pind (@PΓ).
+Proof.
+  apply BD.typing_ind_env.
+
+  1:{ intros. eapply bd_wf_local. eassumption. }
+
+  all: intros ; red ; econstructor ; eauto.
+
+  - clear - X5. induction X5.
+    all: constructor.
+    all: intuition.
+
+  - clear - X0. induction X0.
+    all: constructor.
+    2: auto.
+    destruct p as [? []].
+    eexists. eauto.
+    
+  - remember (fix_context mfix) as Γ'. clear - X1. induction X1.
+    all: constructor.
+    all: intuition.
+  
+  - clear - X0. induction X0.
+    all: constructor.
+    2: auto.
+    destruct p as [? []].
+    eexists. eauto.
+  
+  - remember (fix_context mfix) as Γ'. clear - X1. induction X1.
+    all: constructor.
+    all: intuition.
+    
+  - left.
+    apply PCUICPrincipality.isWfArity_sort.
+    assumption.
+
+  - apply red_cumul.
+    assumption.
+  
+  - have ? : PT.wf Σ.1 by apply bd_wf.
+    eapply isWfArity_or_Type_red ; eauto.
+    eapply validity_term ; eauto.
+
+  - apply red_cumul.
+    assumption.
+    
+  - have ? : PT.wf Σ.1 by apply bd_wf.
+    eapply isWfArity_or_Type_red ; eauto.
+    eapply validity_term ; eauto.
+
+  - apply red_cumul.
+    assumption.
+    
+  - destruct X2 as [ [[? [? []]] ] | [? []]].
+    + left.
+      eexists ; eexists ; split ; eauto.
+      eapply bd_wf_local ; eassumption.
+    + right.
+      eexists.
+      eassumption.
+  
+Qed.
+
+  
+
+
+  
+
+      
